program_logic/auth.v
@@ -13,12 +13,9 @@ Instance authGF_inGF (A : cmraT) `{inGF Λ Σ (authGF A)}
   `{CMRAIdentity A, CMRADiscrete A} : authG Λ Σ A.
 Proof. split; try apply _. apply: inGF_inG. Qed.
 
-Definition auth_own_def `{authG Λ Σ A} (γ : gname) (a : A) : iPropG Λ Σ :=
+Definition auth_own `{authG Λ Σ A} (γ : gname) (a : A) : iPropG Λ Σ :=
   own γ (◯ a).
-(* Perform sealing *)
-Definition auth_own_aux : { x | x = @auth_own_def }. by eexists. Qed.
-Definition auth_own {Λ Σ A Ae a} := proj1_sig auth_own_aux Λ Σ A Ae a.
-Definition auth_own_eq : @auth_own = @auth_own_def := proj2_sig auth_own_aux.
+Typeclasses Opaque auth_own.
 
 Definition auth_inv `{authG Λ Σ A}
     (γ : gname) (φ : A → iPropG Λ Σ) : iPropG Λ Σ :=
@@ -40,17 +37,17 @@ Section auth.
   Implicit Types γ : gname.
 
   Global Instance auth_own_ne n γ : Proper (dist n ==> dist n) (auth_own γ).
-  Proof. rewrite auth_own_eq; solve_proper. Qed.
+  Proof. solve_proper. Qed.
   Global Instance auth_own_proper γ : Proper ((≡) ==> (≡)) (auth_own γ).
-  Proof. by rewrite auth_own_eq; solve_proper. Qed.
+  Proof. solve_proper. Qed.
   Global Instance auth_own_timeless γ a : TimelessP (auth_own γ a).
-  Proof. rewrite auth_own_eq. apply _. Qed.
+  Proof. rewrite /auth_own. apply _. Qed.
 
   Lemma auth_own_op γ a b :
     auth_own γ (a ⋅ b) ≡ (auth_own γ a ★ auth_own γ b)%I.
-  Proof. by rewrite auth_own_eq /auth_own_def -own_op auth_frag_op. Qed.
+  Proof. by rewrite /auth_own -own_op auth_frag_op. Qed.
   Lemma auth_own_valid γ a : auth_own γ a ⊑ ✓ a.
-  Proof. by rewrite auth_own_eq /auth_own_def own_valid auth_validI. Qed.
+  Proof. by rewrite /auth_own own_valid auth_validI. Qed.
 
   Lemma auth_alloc E N a :
     ✓ a → nclose N ⊆ E →
@@ -63,13 +60,13 @@ Section auth.
     trans (▷ auth_inv γ φ ★ auth_own γ a)%I.
     { rewrite /auth_inv -(exist_intro a) later_sep.
       ecancel [▷ φ _]%I.
-      by rewrite -later_intro auth_own_eq -own_op auth_both_op. }
+      by rewrite -later_intro -own_op auth_both_op. }
     rewrite (inv_alloc N) /auth_ctx pvs_frame_r. apply pvs_mono.
     by rewrite always_and_sep_l.
   Qed.
 
   Lemma auth_empty γ E : True ⊑ (|={E}=> auth_own γ ∅).
-  Proof. by rewrite auth_own_eq -own_update_empty. Qed.
+  Proof. by rewrite -own_update_empty. Qed.
 
   Lemma auth_opened E γ a :
     (▷ auth_inv γ φ ★ auth_own γ a)
@@ -78,7 +75,7 @@ Section auth.
     rewrite /auth_inv. rewrite later_exist sep_exist_r. apply exist_elim=>b.
     rewrite later_sep [(▷ own _ _)%I]pvs_timeless !pvs_frame_r. apply pvs_mono.
     rewrite own_valid_l discrete_valid -!assoc. apply const_elim_sep_l=>Hv.
-    rewrite auth_own_eq [(▷φ _ ★ _)%I]comm assoc -own_op.
+    rewrite [(▷φ _ ★ _)%I]comm assoc -own_op.
     rewrite own_valid_r auth_validI /= and_elim_l sep_exist_l sep_exist_r /=.
     apply exist_elim=>a'.
     rewrite left_id -(exist_intro a').
@@ -94,7 +91,7 @@ Section auth.
     (▷ φ (L a ⋅ a') ★ own γ (● (a ⋅ a') ⋅ ◯ a))
     ⊑ (|={E}=> ▷ auth_inv γ φ ★ auth_own γ (L a)).
   Proof.
-    intros HL Hv. rewrite /auth_inv auth_own_eq -(exist_intro (L a ⋅ a')).
+    intros HL Hv. rewrite /auth_inv -(exist_intro (L a ⋅ a')).
     (* TODO it would be really nice to use cancel here *)
     rewrite later_sep [(_ ★ ▷φ _)%I]comm -assoc.
     rewrite -pvs_frame_l. apply sep_mono_r.
